Allow removing the state interpretation from simulation relation

dimsum/iris/expr.v
@@ -9,14 +9,16 @@ Set Default Proof Using "Type".
 Structure mod_lang EV Σ := ModLang {
   mexpr : Type;
   mectx : Type;
+  mstate : Type;
   mfill : mectx → mexpr → mexpr;
   mcomp_ectx : mectx → mectx → mectx;
   mtrans :> mod_trans EV;
   mexpr_rel : mtrans.(m_state) → mexpr → Prop;
-  mstate_interp : mtrans.(m_state) → iProp Σ;
+  mstate_interp : mtrans.(m_state) → option mstate → iProp Σ;
   mfill_comp K1 K2 e : mfill K1 (mfill K2 e) = mfill (mcomp_ectx K1 K2) e
 }.
 Global Arguments mexpr {_ _} _.
+Global Arguments mstate {_ _} _.
 Global Arguments mectx {_ _} _.
 Global Arguments mfill {_ _} _.
 Global Arguments mcomp_ectx {_ _} _.
@@ -26,82 +28,96 @@ Global Arguments mstate_interp {_ _} _ _.
 
 (** * [sim_tgt_expr] *)
 Definition sim_tgt_expr_raw {EV Σ Λ} `{!dimsumGS Σ}
-  (e : mexpr Λ) (Π : option EV → ((m_state Λ → iProp Σ) → iProp Σ) → iProp Σ) : iProp Σ :=
-  (∀ σ, ⌜mexpr_rel Λ σ e⌝ -∗ ord_later_ctx -∗ mstate_interp Λ σ -∗
+  (e : mexpr Λ) (os : option (mstate Λ)) (Π : option EV → ((m_state Λ → iProp Σ) → iProp Σ) → iProp Σ) : iProp Σ :=
+  (∀ σ, ⌜mexpr_rel Λ σ e⌝ -∗ ord_later_ctx -∗ mstate_interp Λ σ os -∗
     σ ≈{ Λ }≈>ₜ Π)%I.
 
-Notation "'TGT' e [{ Π }]" := (sim_tgt_expr_raw e Π%I) (at level 70, Π at level 200,
+Notation "'TGT' e @ ? os [{ Π }]" := (sim_tgt_expr_raw e os Π%I) (at level 70, Π at level 200,
+  format "'[hv' 'TGT'  e  '/' @  ?  os  [{  '[ ' Π  ']' }] ']'") : bi_scope.
+Notation "'TGT' e @ s [{ Π }]" := (sim_tgt_expr_raw e (Some s) Π%I) (at level 70, Π at level 200,
+  format "'[hv' 'TGT'  e  '/' @  s  [{  '[ ' Π  ']' }] ']'") : bi_scope.
+Notation "'TGT' e [{ Π }]" := (sim_tgt_expr_raw e None Π%I) (at level 70, Π at level 200,
   format "'[hv' 'TGT'  e  '/' [{  '[ ' Π  ']' }] ']'") : bi_scope.
 
 Definition sim_tgt_expr {EV Σ Λ} `{!dimsumGS Σ}
-  (e : mexpr Λ) (Π : option EV → ((m_state Λ → iProp Σ) → iProp Σ) → iProp Σ)
-  (Φ : mexpr Λ → (option EV → ((m_state Λ → iProp Σ) → iProp Σ) → iProp Σ) → iProp Σ): iProp Σ :=
-  ∀ K, (∀ e' Π', Φ e' Π' -∗ TGT mfill Λ K e' [{ Π' }]) -∗ TGT mfill Λ K e [{ Π }].
+  (e : mexpr Λ) (os : option (mstate Λ)) (Π : option EV → ((m_state Λ → iProp Σ) → iProp Σ) → iProp Σ)
+  (Φ : mexpr Λ → option (mstate Λ) → (option EV → ((m_state Λ → iProp Σ) → iProp Σ) → iProp Σ) → iProp Σ): iProp Σ :=
+  ∀ K, (∀ e' os' Π', Φ e' os' Π' -∗ TGT mfill Λ K e' @ ? os' [{ Π' }]) -∗ TGT mfill Λ K e @ ? os [{ Π }].
 
-Notation "'TGT' e [{ Π }] {{ Φ } }" := (sim_tgt_expr e Π%I Φ%I)
+Notation "'TGT' e @ ? os [{ Π }] {{ Φ } }" := (sim_tgt_expr e os Π%I Φ%I)
+  (at level 70, Π, Φ at level 200, only parsing) : bi_scope.
+Notation "'TGT' e @ s [{ Π }] {{ Φ } }" := (sim_tgt_expr e (Some s) Π%I Φ%I)
+  (at level 70, Π, Φ at level 200, only parsing) : bi_scope.
+Notation "'TGT' e [{ Π }] {{ Φ } }" := (sim_tgt_expr e None Π%I Φ%I)
   (at level 70, Π, Φ at level 200, only parsing) : bi_scope.
 
-Notation "'TGT' e [{ Π }] {{ e' , Π' , Φ } }" := (sim_tgt_expr e Π%I (λ e' Π', Φ%I))
+Notation "'TGT' e @ ? os [{ Π }] {{ e' , os' , Π' , Φ } }" := (sim_tgt_expr e os Π%I (λ e' os' Π', Φ%I))
   (at level 70, Π, Φ at level 200,
-    format "'[hv' 'TGT'  e  '/' [{  '[ ' Π  ']' }]  {{  '[ ' e' ,  Π' ,  '/' Φ  ']' } } ']'") : bi_scope.
+    format "'[hv' 'TGT'  e  '/' @  ?  os  [{  '[ ' Π  ']' }]  {{  '[ ' e' ,  os' ,  Π' ,  '/' Φ  ']' } } ']'") : bi_scope.
+Notation "'TGT' e @ s [{ Π }] {{ e' , os' , Π' , Φ } }" := (sim_tgt_expr e (Some s) Π%I (λ e' os' Π', Φ%I))
+  (at level 70, Π, Φ at level 200,
+    format "'[hv' 'TGT'  e  '/' @  s  [{  '[ ' Π  ']' }]  {{  '[ ' e' ,  os' ,  Π' ,  '/' Φ  ']' } } ']'") : bi_scope.
+Notation "'TGT' e [{ Π }] {{ e' , os' , Π' , Φ } }" := (sim_tgt_expr e None Π%I (λ e' os' Π', Φ%I))
+  (at level 70, Π, Φ at level 200,
+    format "'[hv' 'TGT'  e  '/' [{  '[ ' Π  ']' }]  {{  '[ ' e' ,  os' ,  Π' ,  '/' Φ  ']' } } ']'") : bi_scope.
 
 Section sim_tgt.
 Context {EV} {Σ} {Λ : mod_lang EV Σ} `{!dimsumGS Σ}.
 Implicit Types (e : mexpr Λ).
 
-Lemma sim_tgt_expr_raw_step e Π:
-  (∀ σ κ Pσ, ⌜mexpr_rel Λ σ e⌝ -∗ ⌜Λ.(m_step) σ κ Pσ⌝ -∗ mstate_interp Λ σ ={∅}=∗ ▷ₒ
+Lemma sim_tgt_expr_raw_step e Π os :
+  (∀ σ κ Pσ, ⌜mexpr_rel Λ σ e⌝ -∗ ⌜Λ.(m_step) σ κ Pσ⌝ -∗ mstate_interp Λ σ os ={∅}=∗ ▷ₒ
       (Π κ (λ P', ∃ σ', ⌜Pσ σ'⌝ ∗ P' σ') ∨
-         ∃ σ' e', ⌜κ = None⌝ ∗ ⌜Pσ σ'⌝ ∗ ⌜mexpr_rel Λ σ' e'⌝ ∗ mstate_interp Λ σ' ∗ TGT e' [{ Π }])) -∗
-  TGT e [{ Π }].
+         ∃ os' σ' e', ⌜κ = None⌝ ∗ ⌜Pσ σ'⌝ ∗ ⌜mexpr_rel Λ σ' e'⌝ ∗ mstate_interp Λ σ' os' ∗ TGT e' @ ? os' [{ Π }])) -∗
+  TGT e @ ? os [{ Π }].
 Proof.
   iIntros "HΠ" (σ ?) "#??".
   iApply sim_tgt_step. iIntros (???). iMod ("HΠ" with "[//] [//] [$]") as "Hsim". do 2 iModIntro.
-  iDestruct "Hsim" as "[$|(%&%&%&%&%&?&Hsim)]". iRight. iExists _. iSplit; [done|]. iSplit; [done|].
+  iDestruct "Hsim" as "[$|(%&%&%&%&%&%&?&Hsim)]". iRight. iExists _. iSplit; [done|]. iSplit; [done|].
   by iApply "Hsim".
 Qed.
 
-Lemma sim_tgt_expr_raw_elim e Π σ :
+Lemma sim_tgt_expr_raw_elim e Π σ os :
   mexpr_rel Λ σ e →
-  mstate_interp Λ σ -∗
-  TGT e [{ Π }] -∗
+  mstate_interp Λ σ os -∗
+  TGT e @ ? os [{ Π }] -∗
   σ ≈{Λ}≈>ₜ Π.
 Proof. iIntros (?) "Hσ He". iApply sim_tgt_ctx. iIntros "#?". by iApply "He". Qed.
 
-Lemma sim_tgt_expr_ctx e Π Φ :
-  (ord_later_ctx -∗ TGT e [{ Π }] {{ Φ }}) -∗
-  TGT e [{ Π }] {{ Φ }}.
+Lemma sim_tgt_expr_ctx e Π Φ os :
+  (ord_later_ctx -∗ TGT e @ ? os [{ Π }] {{ Φ }}) -∗
+  TGT e @ ? os [{ Π }] {{ Φ }}.
 Proof.
   iIntros "Hsim" (?) "HΦ". iIntros (??) "#?". iApply ("Hsim" with "[$] [$] [//] [$]").
 Qed.
 
-Lemma fupd_sim_tgt_expr e Π Φ :
-  (|={∅}=> TGT e [{ Π }] {{ Φ }}) -∗
-  TGT e [{ Π }] {{ Φ }}.
+Lemma fupd_sim_tgt_expr e Π Φ os :
+  (|={∅}=> TGT e @ ? os [{ Π }] {{ Φ }}) -∗
+  TGT e @ ? os [{ Π }] {{ Φ }}.
 Proof.
   iIntros "Hsim" (?) "HΦ". iIntros (??) "#??". iApply fupd_sim_tgt. iApply ("Hsim" with "[$] [//] [//] [$]").
 Qed.
 
-Lemma sim_tgt_expr_bi_mono e Π Φ :
-  (TGT e [{ λ κ, bi_mono1 (Π κ) }] {{ Φ }}) -∗
-  TGT e [{ Π }] {{ Φ }}.
+Lemma sim_tgt_expr_bi_mono e Π Φ os :
+  (TGT e @ ? os [{ λ κ, bi_mono1 (Π κ) }] {{ Φ }}) -∗
+  TGT e @ ? os [{ Π }] {{ Φ }}.
 Proof.
   iIntros "Hsim" (?) "HΦ". iIntros (??) "#??". iApply sim_tgt_bi_mono1.
   iApply ("Hsim" with "[$] [//] [//] [$]").
 Qed.
 
-Lemma sim_tgt_expr_bind K e Π Φ :
-  TGT e [{ Π }] {{ e', Π', TGT mfill Λ K e' [{ Π' }] {{ Φ }} }} -∗
-  TGT mfill Λ K e [{ Π }] {{ Φ }}.
+Lemma sim_tgt_expr_bind K e Π Φ os :
+  TGT e @ ? os [{ Π }] {{ e', os', Π', TGT mfill Λ K e' @ ? os' [{ Π' }] {{ Φ }} }} -∗
+  TGT mfill Λ K e @ ? os [{ Π }] {{ Φ }}.
 Proof.
   iIntros "Hsim" (?) "HΦ". rewrite mfill_comp. iApply "Hsim".
-  iIntros (??) "Htgt". rewrite -mfill_comp. by iApply "Htgt".
+  iIntros (???) "Htgt". rewrite -mfill_comp. by iApply "Htgt".
 Qed.
 
-Lemma sim_tgt_expr_wand1 e Π Π' Φ  :
-  TGT e [{ Π' }] {{ Φ }} -∗
+Lemma sim_tgt_expr_wand1 e Π Π' Φ os :
+  TGT e @ ? os [{ Π' }] {{ Φ }} -∗
   (∀ κ P, Π' κ P -∗ Π κ P) -∗
-  TGT e [{ Π }] {{ Φ }}.
+  TGT e @ ? os [{ Π }] {{ Φ }}.
 Proof.
   iIntros "Hsim Hwand" (?) "HΦ".
   iIntros (??) "#? Hσ".
@@ -109,61 +125,61 @@ Proof.
   iApply ("Hsim" with "[$] [//] [$] [$]").
 Qed.
 
-Lemma sim_tgt_expr_wand e Π Φ Φ' :
-  TGT e [{ Π }] {{ Φ' }} -∗
-  (∀ e' Π', Φ' e' Π' -∗ Φ e' Π') -∗
-  TGT e [{ Π }] {{ Φ }}.
-Proof. iIntros "Hsim Hwand" (?) "HΦ". iApply "Hsim". iIntros (??) "Hsim". iApply "HΦ". by iApply "Hwand". Qed.
+Lemma sim_tgt_expr_wand e Π Φ Φ' os :
+  TGT e @ ? os [{ Π }] {{ Φ' }} -∗
+  (∀ e' os' Π', Φ' e' os' Π' -∗ Φ e' os' Π') -∗
+  TGT e @ ? os [{ Π }] {{ Φ }}.
+Proof. iIntros "Hsim Hwand" (?) "HΦ". iApply "Hsim". iIntros (???) "Hsim". iApply "HΦ". by iApply "Hwand". Qed.
 
-Lemma sim_tgt_expr_stop1 e Π Φ :
-  (∀ σ, σ ⤇ₜ (λ Π', TGT e [{ Π' }] {{ Φ }}) -∗ Π None (λ P, P σ)) -∗
-  TGT e [{ Π }] {{ Φ }}.
+Lemma sim_tgt_expr_stop1 e Π Φ os :
+  (∀ σ, σ ⤇ₜ (λ Π', TGT e @ ? os [{ Π' }] {{ Φ }}) -∗ Π None (λ P, P σ)) -∗
+  TGT e @ ? os [{ Π }] {{ Φ }}.
 Proof.
   iIntros "HΦ" (?) "HF". iIntros (??) "??".
   iApply sim_tgt_stop. iApply "HΦ". iIntros (?) "Hsim".
   iApply ("Hsim" with "[$] [//] [$] [$]").
 Qed.
 
-Lemma sim_tgt_expr_stop2 e Π Φ :
-  Φ e Π -∗ TGT e [{ Π }] {{ Φ }}.
+Lemma sim_tgt_expr_stop2 e Π Φ os :
+  Φ e os Π -∗ TGT e @ ? os [{ Π }] {{ Φ }}.
 Proof. iIntros "HΦ" (?) "HF". by iApply "HF". Qed.
 
-Lemma sim_tgt_expr_elim K e Π σ :
+Lemma sim_tgt_expr_elim os K e Π σ :
   mexpr_rel Λ σ (mfill Λ K e) →
-  mstate_interp Λ σ -∗
-  TGT e [{ Π }] {{ _, _, False }} -∗
+  mstate_interp Λ σ os -∗
+  TGT e @ ? os [{ Π }] {{ _, _, _, False }} -∗
   σ ≈{Λ}≈>ₜ Π.
 Proof.
   iIntros (?) "Hσ He". iApply (sim_tgt_expr_raw_elim with "[$]"); [done|].
-  iApply "He". by iIntros (??) "?".
+  iApply "He". by iIntros (???) "?".
 Qed.
 
-Lemma sim_tgt_expr_step_None e Π Φ :
-  (∀ K σ κ Pσ, ⌜mexpr_rel Λ σ (mfill Λ K e)⌝ -∗ ⌜Λ.(m_step) σ κ Pσ⌝ -∗ mstate_interp Λ σ ={∅}=∗ ▷ₒ
-      (∃ σ' e', ⌜κ = None⌝ ∗ ⌜Pσ σ'⌝ ∗ ⌜mexpr_rel Λ σ' (mfill Λ K e')⌝ ∗ mstate_interp Λ σ' ∗ TGT e' [{ Π }] {{Φ}})) -∗
-  TGT e [{ Π }] {{ Φ }}.
+Lemma sim_tgt_expr_step_None e Π Φ os :
+  (∀ K σ κ Pσ, ⌜mexpr_rel Λ σ (mfill Λ K e)⌝ -∗ ⌜Λ.(m_step) σ κ Pσ⌝ -∗ mstate_interp Λ σ os ={∅}=∗ ▷ₒ
+      (∃ os' σ' e', ⌜κ = None⌝ ∗ ⌜Pσ σ'⌝ ∗ ⌜mexpr_rel Λ σ' (mfill Λ K e')⌝ ∗ mstate_interp Λ σ' os' ∗ TGT e' @ ? os' [{ Π }] {{Φ}})) -∗
+  TGT e @ ? os [{ Π }] {{ Φ }}.
 Proof.
   iIntros "Hs" (?) "HΦ". iApply sim_tgt_expr_raw_step. iIntros (?????) "?".
   iMod ("Hs" with "[//] [//] [$]") as "Hs". do 2 iModIntro. iRight.
-  iDestruct "Hs" as (?????) "[? Hsim]". iExists _, _. iSplit; [done|]. iSplit; [done|]. iSplit; [done|].
+  iDestruct "Hs" as (??????) "[? Hsim]". iExists _, _, _. iSplit; [done|]. iSplit; [done|]. iSplit; [done|].
   iFrame. by iApply "Hsim".
 Qed.
 
-Lemma sim_tgt_expr_step e Φ Π :
-  (∀ K σ κ Pσ, ⌜mexpr_rel Λ σ (mfill Λ K e)⌝ -∗ ⌜m_step Λ σ κ Pσ⌝ -∗ mstate_interp Λ σ ={∅}=∗ ▷ₒ
+Lemma sim_tgt_expr_step e Φ Π os :
+  (∀ K σ κ Pσ, ⌜mexpr_rel Λ σ (mfill Λ K e)⌝ -∗ ⌜m_step Λ σ κ Pσ⌝ -∗ mstate_interp Λ σ os ={∅}=∗ ▷ₒ
      Π κ (λ P, ∃ σ', ⌜Pσ σ'⌝ ∗
-       ((∀ e',
+       ((∀ os' e',
            ⌜mexpr_rel Λ σ' (mfill Λ K e')⌝ -∗
-           mstate_interp Λ σ' -∗
-           σ' ⤇ₜ λ Π', TGT e' [{ Π' }] {{ Φ }}) -∗
+           mstate_interp Λ σ' os' -∗
+           σ' ⤇ₜ λ Π', TGT e' @ ? os' [{ Π' }] {{ Φ }}) -∗
           P σ'))) -∗
-  TGT e [{ Π }] {{ Φ }}.
+  TGT e @ ? os [{ Π }] {{ Φ }}.
 Proof.
   iIntros "Hsim" (?). iIntros "HΦ" (??) "#? Hσ".
   iApply sim_tgt_bi_mono1. iApply sim_tgt_step_end. iIntros (???). iMod ("Hsim" with "[//] [//] [$]") as "Hsim".
   do 2 iModIntro. iApply (bi_mono1_intro with "Hsim"). iIntros (?) "[% [% Hsim]]".
   iExists _. iSplit; [done|]. iApply "Hsim".
-  iIntros (??) "?". iIntros (?) "Hsim". iApply (sim_tgt_expr_raw_elim with "[$]"); [done|].
+  iIntros (???) "?". iIntros (?) "Hsim". iApply (sim_tgt_expr_raw_elim with "[$]"); [done|].
   by iApply "Hsim".
 Qed.
 
@@ -171,76 +187,88 @@ End sim_tgt.
 
 (** * [sim_src_expr] *)
 Definition sim_src_expr_raw {EV Σ Λ} `{!dimsumGS Σ}
-  (e : mexpr Λ) (Π : option EV → m_state Λ → iProp Σ) : iProp Σ :=
-  (∀ σ, ⌜mexpr_rel Λ σ e⌝ -∗ ord_later_ctx -∗ mstate_interp Λ σ -∗
+  (e : mexpr Λ) (os : option (mstate Λ)) (Π : option EV → m_state Λ → iProp Σ) : iProp Σ :=
+  (∀ σ, ⌜mexpr_rel Λ σ e⌝ -∗ ord_later_ctx -∗ mstate_interp Λ σ os -∗
     σ ≈{ Λ }≈>ₛ Π)%I.
 
-Notation "'SRC' e [{ Π }]" := (sim_src_expr_raw e Π%I) (at level 70, Π at level 200,
+Notation "'SRC' e @ ? os [{ Π }]" := (sim_src_expr_raw e os Π%I) (at level 70, Π at level 200,
+  format "'[hv' 'SRC'  e  '/' @  ?  os  [{  '[ ' Π  ']' }] ']'") : bi_scope.
+Notation "'SRC' e @ s [{ Π }]" := (sim_src_expr_raw e (Some s) Π%I) (at level 70, Π at level 200,
+  format "'[hv' 'SRC'  e  '/' @  s  [{  '[ ' Π  ']' }] ']'") : bi_scope.
+Notation "'SRC' e [{ Π }]" := (sim_src_expr_raw e None Π%I) (at level 70, Π at level 200,
   format "'[hv' 'SRC'  e  '/' [{  '[ ' Π  ']' }] ']'") : bi_scope.
 
 Definition sim_src_expr {EV Σ Λ} `{!dimsumGS Σ}
-  (e : mexpr Λ) (Π : option EV → m_state Λ → iProp Σ)
-  (Φ : mexpr Λ → (option EV → m_state Λ → iProp Σ) → iProp Σ): iProp Σ :=
-  ∀ K, (∀ e' Π', Φ e' Π' -∗ SRC mfill Λ K e' [{ Π' }]) -∗ SRC mfill Λ K e [{ Π }].
+  (e : mexpr Λ) (os : option (mstate Λ)) (Π : option EV → m_state Λ → iProp Σ)
+  (Φ : mexpr Λ → option (mstate Λ) → (option EV → m_state Λ → iProp Σ) → iProp Σ): iProp Σ :=
+  ∀ K, (∀ e' os' Π', Φ e' os' Π' -∗ SRC mfill Λ K e' @ ? os' [{ Π' }]) -∗ SRC mfill Λ K e @ ? os [{ Π }].
 
-Notation "'SRC' e [{ Π }] {{ Φ } }" := (sim_src_expr e Π%I Φ%I)
+Notation "'SRC' e @ ? os [{ Π }] {{ Φ } }" := (sim_src_expr e os Π%I Φ%I)
+  (at level 70, Π, Φ at level 200, only parsing) : bi_scope.
+Notation "'SRC' e @ s [{ Π }] {{ Φ } }" := (sim_src_expr e (Some s) Π%I Φ%I)
+  (at level 70, Π, Φ at level 200, only parsing) : bi_scope.
+Notation "'SRC' e [{ Π }] {{ Φ } }" := (sim_src_expr e None Π%I Φ%I)
   (at level 70, Π, Φ at level 200, only parsing) : bi_scope.
 
-Notation "'SRC' e [{ Π }] {{ e' , Π' , Φ } }" := (sim_src_expr e Π%I (λ e' Π', Φ%I)) (at level 70, Π, Φ at level 200,
-  format "'[hv' 'SRC'  e  '/' [{  '[ ' Π  ']' }]  {{  '[ ' e' ,  Π' ,  '/' Φ  ']' } } ']'") : bi_scope.
+Notation "'SRC' e @ ? os [{ Π }] {{ e' , os' , Π' , Φ } }" := (sim_src_expr e os Π%I (λ e' os' Π', Φ%I)) (at level 70, Π, Φ at level 200,
+  format "'[hv' 'SRC'  e  '/' @  ?  os  [{  '[ ' Π  ']' }]  {{  '[ ' e' ,  os' ,  Π' ,  '/' Φ  ']' } } ']'") : bi_scope.
+Notation "'SRC' e @ s [{ Π }] {{ e' , os' , Π' , Φ } }" := (sim_src_expr e (Some s) Π%I (λ e' os' Π', Φ%I)) (at level 70, Π, Φ at level 200,
+  format "'[hv' 'SRC'  e  '/' @  s  [{  '[ ' Π  ']' }]  {{  '[ ' e' ,  os' ,  Π' ,  '/' Φ  ']' } } ']'") : bi_scope.
+Notation "'SRC' e [{ Π }] {{ e' , os' , Π' , Φ } }" := (sim_src_expr e None Π%I (λ e' os' Π', Φ%I)) (at level 70, Π, Φ at level 200,
+  format "'[hv' 'SRC'  e  '/' [{  '[ ' Π  ']' }]  {{  '[ ' e' ,  os' ,  Π' ,  '/' Φ  ']' } } ']'") : bi_scope.
 
 Section sim_src.
 Context {EV} {Σ} {Λ : mod_lang EV Σ} `{!dimsumGS Σ}.
 Implicit Types (e : mexpr Λ).
 
-Lemma sim_src_expr_raw_step e Π:
-  (∀ σ, ⌜mexpr_rel Λ σ e⌝ -∗ mstate_interp Λ σ ==∗
+Lemma sim_src_expr_raw_step e Π os :
+  (∀ σ, ⌜mexpr_rel Λ σ e⌝ -∗ mstate_interp Λ σ os ==∗
     ∃ κ Pσ, ⌜m_step Λ σ κ Pσ⌝ ∗
      ∀ σ', ⌜Pσ σ'⌝ ={∅}=∗ if κ is Some _ then Π κ σ' else
-       ∃ e', ⌜mexpr_rel Λ σ' e'⌝ ∗ mstate_interp Λ σ' ∗ SRC e' [{ Π }]) -∗
-  SRC e [{ Π }].
+       ∃ os' e', ⌜mexpr_rel Λ σ' e'⌝ ∗ mstate_interp Λ σ' os' ∗ SRC e' @ ? os' [{ Π }]) -∗
+  SRC e @ ? os [{ Π }].
 Proof.
   iIntros "HΠ" (σ ?) "#??". iApply fupd_sim_src.
   iMod ("HΠ" with "[//] [$]") as (???) "HΠ". iModIntro.
   iApply sim_src_step; [done..|]. iIntros (??).
   iMod ("HΠ" with "[//]") as "HΠ". case_match; [done|]. iModIntro.
-  iDestruct ("HΠ") as (??) "[? Hsim]".
+  iDestruct ("HΠ") as (???) "[? Hsim]".
   by iApply "Hsim".
 Qed.
 
-Lemma sim_src_expr_raw_elim e Π σ :
+Lemma sim_src_expr_raw_elim e Π σ os :
   mexpr_rel Λ σ e →
-  mstate_interp Λ σ -∗
-  SRC e [{ Π }] -∗
+  mstate_interp Λ σ os -∗
+  SRC e @ ? os [{ Π }] -∗
   σ ≈{Λ}≈>ₛ Π.
 Proof. iIntros (?) "Hσ He". iApply sim_src_ctx. iIntros "#?". by iApply "He". Qed.
 
-Lemma fupd_sim_src_expr e Π Φ :
-  (|={∅}=> SRC e [{ Π }] {{ Φ }}) -∗
-  SRC e [{ Π }] {{ Φ }}.
+Lemma fupd_sim_src_expr e Π Φ os :
+  (|={∅}=> SRC e @ ? os [{ Π }] {{ Φ }}) -∗
+  SRC e @ ? os [{ Π }] {{ Φ }}.
 Proof.
   iIntros "Hsim" (?) "HΦ". iIntros (??) "#??". iApply fupd_sim_src. iApply ("Hsim" with "[$] [//] [//] [$]").
 Qed.
 
-Lemma sim_src_expr_ctx e Π Φ :
-  (ord_later_ctx -∗ SRC e [{ Π }] {{ Φ }}) -∗
-  SRC e [{ Π }] {{ Φ }}.
+Lemma sim_src_expr_ctx e Π Φ os :
+  (ord_later_ctx -∗ SRC e @ ? os [{ Π }] {{ Φ }}) -∗
+  SRC e @ ? os [{ Π }] {{ Φ }}.
 Proof.
   iIntros "Hsim" (?) "HΦ". iIntros (??) "#?". iApply ("Hsim" with "[$] [$] [//] [$]").
 Qed.
 
-Lemma sim_src_expr_bind e Π Φ K :
-  SRC e [{ Π }] {{ e', Π', SRC mfill Λ K e' [{ Π' }] {{ Φ }} }} -∗
-  SRC mfill Λ K e [{ Π }] {{ Φ }}.
+Lemma sim_src_expr_bind e Π Φ K os :
+  SRC e @ ? os [{ Π }] {{ e', os', Π', SRC mfill Λ K e' @ ? os' [{ Π' }] {{ Φ }} }} -∗
+  SRC mfill Λ K e @ ? os [{ Π }] {{ Φ }}.
 Proof.
   iIntros "Hsim" (?) "HΦ". rewrite mfill_comp. iApply "Hsim".
-  iIntros (??) "Htgt". rewrite -mfill_comp. by iApply "Htgt".
+  iIntros (???) "Htgt". rewrite -mfill_comp. by iApply "Htgt".
 Qed.
 
-Lemma sim_src_expr_wand1 e Π Π' Φ  :
-  SRC e [{ Π' }] {{ Φ }} -∗
+Lemma sim_src_expr_wand1 e Π Π' Φ os :
+  SRC e @ ? os [{ Π' }] {{ Φ }} -∗
   (∀ κ P, Π' κ P -∗ Π κ P) -∗
-  SRC e [{ Π }] {{ Φ }}.
+  SRC e @ ? os [{ Π }] {{ Φ }}.
 Proof.
   iIntros "Hsim Hwand" (?) "HΦ".
   iIntros (??) "#? Hσ".
@@ -248,63 +276,63 @@ Proof.
   iApply ("Hsim" with "[$] [//] [$] [$]").
 Qed.
 
-Lemma sim_src_expr_wand e Π Φ Φ' :
-  SRC e [{ Π }] {{ Φ' }} -∗
-  (∀ e' Π', Φ' e' Π' -∗ Φ e' Π') -∗
-  SRC e [{ Π }] {{ Φ }}.
-Proof. iIntros "Hsim Hwand" (?) "HΦ". iApply "Hsim". iIntros (??) "Hsim". iApply "HΦ". by iApply "Hwand". Qed.
+Lemma sim_src_expr_wand e Π Φ Φ' os :
+  SRC e @ ? os [{ Π }] {{ Φ' }} -∗
+  (∀ e' os' Π', Φ' e' os' Π' -∗ Φ e' os' Π') -∗
+  SRC e @ ? os [{ Π }] {{ Φ }}.
+Proof. iIntros "Hsim Hwand" (?) "HΦ". iApply "Hsim". iIntros (???) "Hsim". iApply "HΦ". by iApply "Hwand". Qed.
 
-Lemma sim_src_expr_stop1 e Π Φ :
-  (∀ σ, σ ⤇ₛ (λ Π', SRC e [{ Π' }] {{ Φ }}) -∗ Π None σ) -∗
-  SRC e [{ Π }] {{ Φ }}.
+Lemma sim_src_expr_stop1 e Π Φ os :
+  (∀ σ, σ ⤇ₛ (λ Π', SRC e @ ? os [{ Π' }] {{ Φ }}) -∗ Π None σ) -∗
+  SRC e @ ? os [{ Π }] {{ Φ }}.
 Proof.
   iIntros "HΦ" (?) "HF". iIntros (??) "??".
   iApply sim_src_stop. iApply "HΦ". iIntros (?) "Hsim".
   iApply ("Hsim" with "[$] [//] [$] [$]").
 Qed.
 
-Lemma sim_src_expr_stop2 e Π Φ :
-  Φ e Π -∗ SRC e [{ Π }] {{ Φ }}.
+Lemma sim_src_expr_stop2 e Π Φ os :
+  Φ e os Π -∗ SRC e @ ? os [{ Π }] {{ Φ }}.
 Proof. iIntros "HΦ" (?) "HF". by iApply "HF". Qed.
 
-Lemma sim_src_expr_elim e Π σ K :
+Lemma sim_src_expr_elim os e Π σ K :
   mexpr_rel Λ σ (mfill Λ K e) →
-  mstate_interp Λ σ -∗
-  SRC e [{ Π }] {{ _, _, False }} -∗
+  mstate_interp Λ σ os -∗
+  SRC e @ ? os [{ Π }] {{ _, _, _, False }} -∗
   σ ≈{Λ}≈>ₛ Π.
 Proof.
   iIntros (?) "Hσ He". iApply (sim_src_expr_raw_elim with "[$]"); [done|].
-  iApply "He". by iIntros (??) "?".
+  iApply "He". by iIntros (???) "?".
 Qed.
 
-Lemma sim_src_expr_step_None e Π Φ :
-  (∀ K σ, ⌜mexpr_rel Λ σ (mfill Λ K e)⌝ -∗ mstate_interp Λ σ ==∗
+Lemma sim_src_expr_step_None e Π Φ os :
+  (∀ K σ, ⌜mexpr_rel Λ σ (mfill Λ K e)⌝ -∗ mstate_interp Λ σ os ==∗
     ∃ Pσ, ⌜m_step Λ σ None Pσ⌝ ∗
-     ∀ σ', ⌜Pσ σ'⌝ ={∅}=∗ ∃ e', ⌜mexpr_rel Λ σ' (mfill Λ K e')⌝ ∗
-       mstate_interp Λ σ' ∗ SRC e' [{ Π }] {{ Φ }}) -∗
-  SRC e [{ Π }] {{ Φ }}.
+     ∀ σ', ⌜Pσ σ'⌝ ={∅}=∗ ∃ os' e', ⌜mexpr_rel Λ σ' (mfill Λ K e')⌝ ∗
+       mstate_interp Λ σ' os' ∗ SRC e' @ ? os' [{ Π }] {{ Φ }}) -∗
+  SRC e @ ? os [{ Π }] {{ Φ }}.
 Proof.
   iIntros "Hs" (?) "HΦ". iApply sim_src_expr_raw_step. iIntros (??) "?".
   iMod ("Hs" with "[//] [$]") as (??) "Hs". iModIntro. iExists _, _. iSplit; [done|].
-  iIntros (??). iMod ("Hs" with "[//]") as (??) "[$ Hs]". iModIntro. iExists _. iSplit; [done|].
+  iIntros (??). iMod ("Hs" with "[//]") as (???) "[? Hs]". iModIntro. iExists _, _. iFrame. iSplit; [done|].
   by iApply "Hs".
 Qed.
 
-Lemma sim_src_expr_step e Φ Π :
-  (∀ K σ, ⌜mexpr_rel Λ σ (mfill Λ K e)⌝ -∗ mstate_interp Λ σ ==∗
+Lemma sim_src_expr_step e Φ Π os :
+  (∀ K σ, ⌜mexpr_rel Λ σ (mfill Λ K e)⌝ -∗ mstate_interp Λ σ os ==∗
      ∃ κ' Pσ_s, ⌜m_step Λ σ κ' Pσ_s⌝ ∗
        ∀ σ', ⌜Pσ_s σ'⌝ ={∅}=∗
-          ((∀ e',
+          ((∀ os' e',
               ⌜mexpr_rel Λ σ' (mfill Λ K e')⌝ -∗
-              mstate_interp Λ σ' -∗
-              σ' ⤇ₛ λ Π', SRC e' [{ Π' }] {{ Φ }}) -∗
+              mstate_interp Λ σ' os' -∗
+              σ' ⤇ₛ λ Π', SRC e' @ ? os' [{ Π' }] {{ Φ }}) -∗
           Π κ' σ')) -∗
-  SRC e [{ Π }] {{ Φ }}.
+  SRC e @ ? os [{ Π }] {{ Φ }}.
 Proof.
   iIntros "He" (?). iIntros "HΦ" (??) "#? Hσ". iApply fupd_sim_src.
   iMod ("He" with "[//] [$]") as (???) "Hsim". iModIntro.
   iApply sim_src_step_end; [done|]. iIntros (??). iMod ("Hsim" with "[//]") as "Hsim".
-  iModIntro. iApply "Hsim". iIntros (??) "?". iIntros (?) "Hsim".
+  iModIntro. iApply "Hsim". iIntros (???) "?". iIntros (?) "Hsim".
   iApply (sim_src_expr_raw_elim with "[$]"); [done|].
   by iApply "Hsim".
 Qed.
